tests/coq/ERC20/Theory.v
@@ -31,6 +31,48 @@ Definition transfer_to map (from : address) (amt : Z) :=
 
 Definition transfer map from to amt := transfer_to (transfer_from map from amt) to amt.
 
+Definition transfer' map from to amt := transfer_from (transfer_to map to amt) from amt.
+
+Inductive transferRelation from to amt (map : address -> Z) (map' : address -> Z) : Prop:= 
+  | transferEqC:
+      from <> to
+  -> (forall p, p <> from -> p <> to -> map p = map' p)
+  -> map from = map' from + amt 
+  -> map to + amt= map' to
+  -> transferRelation from to amt map map'
+  | transferNeqC:
+      from = to
+  -> (forall p, map p = map' p)
+  -> transferRelation from to amt map map'.
+
+Inductive transferStateRelation from to amt s s' : Prop:= 
+  | transferStateC: 
+    transferRelation from to amt (balanceOf s) (balanceOf s')
+    -> transferStateRelation from to amt s s'.
+
+Inductive mintRelation to amt map (map' : address -> Z) : Prop:= 
+  | mintC: 
+  map to + amt= map' to
+  -> (forall p, p <> to -> map p = map' p)
+  ->  mintRelation to amt map map'.
+
+Inductive mintStateRelation to amt s s' : Prop:= 
+  | mintStateC: 
+    mintRelation to amt (balanceOf s) (balanceOf s')
+    -> mintStateRelation to amt s s'.
+
+Inductive burnRelation from amt map (map' : address -> Z) : Prop:= 
+  | burnC: 
+      map from = map' from + amt
+  -> (forall p, p <> from -> map p = map' p)
+  ->  burnRelation from amt map map'.
+
+Inductive burnStateRelation from amt s s' : Prop:= 
+  | burnStateC: 
+    burnRelation from amt (balanceOf s) (balanceOf s')
+    -> burnStateRelation from amt s s'.
+
+
 Lemma balanceOf_sum_f_eq f f' addr acc :
   (forall x, x <= Z.of_nat addr -> f x = f' x) ->
   balanceOf_sum' f addr acc = balanceOf_sum' f' addr acc.
@@ -110,51 +152,51 @@ Proof.
     rewrite Z.eqb_sym, H. reflexivity.
 Qed.
 
-Lemma balanceOf_sum_transfer_to map to amt addr acc :
+Lemma balanceOf_sum_burnFrom map from amt addr acc map' :
+  0 <= from ->
+  burnRelation from amt map map' ->
+  balanceOf_sum' map' addr acc =
+  if (Z.to_nat from <=? addr)%nat then balanceOf_sum' map addr acc - amt else balanceOf_sum' map addr acc.
+Proof.
+  intros Hleq1 Hburn.
+  destruct Hburn as [HburnFrom HburnElse].
+  erewrite balanceOf_sum_thm with (f := map') (f' := map) (x := from); eauto.
+
+  - destruct (Z.to_nat from <=? addr)%nat eqn:Hleq.
+    lia. lia.
+
+  - intros. rewrite Z.eq_sym_iff. apply HburnElse. lia.
+Qed.
+
+Lemma balanceOf_sum_mintTo map to amt addr acc map':
   0 <= to ->
-  balanceOf_sum' (transfer_to map to amt) addr acc =
+  mintRelation to amt map map' ->
+  balanceOf_sum' map' addr acc =
   if (Z.to_nat to <=? addr)%nat then balanceOf_sum' map addr acc + amt else balanceOf_sum' map addr acc.
 Proof.
-  intros Hleq1.
-  erewrite balanceOf_sum_thm with (f := transfer_to map to amt) (f' := map) (x := to); eauto.
+  intros Hleq1 Hmint.
+  destruct Hmint as [HmintFrom HmintElse].
+  erewrite balanceOf_sum_thm with (f := map') (f' := map) (x := to); eauto.
 
   - destruct (Z.to_nat to <=? addr)%nat eqn:Hleq.
+    lia. lia.
 
-    unfold transfer_to. rewrite Z.eqb_refl. lia.
-
-    reflexivity.
-
-  - intros. unfold transfer_to. eapply Z.eqb_neq in H.
-    rewrite Z.eqb_sym, H. reflexivity.
+  - intros. rewrite Z.eq_sym_iff. apply HmintElse. lia.
 Qed.
 
+Ltac convert_neq :=
+  repeat match goal with
+    [ H : _ <> _ |- _ ] => let H_og := fresh H "'" in eapply not_eq_sym in H as H_og; eapply Z.eqb_neq in H; eapply Z.eqb_neq in H_og
+  end.
 
-Theorem transfer_thm map from to amt addr acc:
-  to <> from ->
-  0 <= from <= Z.of_nat addr ->
-  0 <= to <= Z.of_nat addr ->
-  balanceOf_sum' (transfer map from to amt) addr acc  = balanceOf_sum' map addr acc.
-Proof.
-  intros Hneq Hleq1 Hleq2.
-  unfold transfer.
-
-  rewrite balanceOf_sum_transfer_to; [ | lia ].
-  rewrite leb_correct; [ | lia ].
-
-  rewrite balanceOf_sum_transfer_from; [ | lia ].
-  rewrite leb_correct; [ | lia ].
-
-  lia.
-Qed.
+Ltac convert_eq :=
+  repeat match goal with
+    [ H : _ = _ |- _ ] => let H_og := fresh H "'" in eapply eq_sym in H as H_og; eapply Z.eqb_eq in H; eapply Z.eqb_eq in H_og
+  end.
 
 Ltac destructAnds :=
   repeat match goal with
     [ H : _ /\ _ |- _ ] => destruct H
-  end.
-
-Ltac convert_neq :=
-  repeat match goal with
-    [ H : _ <> _ |- _ ] => eapply not_eq_sym in H; eapply Z.eqb_neq in H
   end.
 
 Ltac rewrite_eqs :=
@@ -162,81 +204,130 @@ Ltac rewrite_eqs :=
     [ H : _ =? _ = _ |- _ ] => rewrite H
   end.
 
-Lemma balances_after_transfer ENV STATE src dst amount :
+Theorem transfer_burn_mint from to amt map imap map':
+  0 <= from ->
+  0 <= to ->
+  transferRelation from to amt map map' ->
+  imap = (fun p => if p =? from then map p - amt else map p) ->
+  (burnRelation from amt map imap
+  /\ mintRelation to amt imap map').
+Proof.
+  intros Hleq1 Hleq2 Htransfer Himap.
+  rewrite Himap in *.
+  split.
+  - constructor.
+    + rewrite Z.eqb_refl. lia.
+    + destruct Htransfer; intros p Hpleq; convert_neq; rewrite_eqs; reflexivity.
+  - constructor.
+    + destruct Htransfer.
+      * convert_neq. rewrite_eqs. assumption.
+      * convert_eq. rewrite_eqs. rewrite H0. lia.
+    + destruct Htransfer; intros p Hpneq.
+      * destruct (p =? from) eqn:HpFrom.
+        -- apply Z.eqb_eq in HpFrom. rewrite HpFrom. lia.
+        -- apply H0; [apply Z.eqb_neq| ]; assumption.
+      * convert_neq. rewrite H. rewrite_eqs. rewrite H0. lia.
+Qed.
+
+
+Theorem transfer_thm map from to amt addr acc: forall map',
+  to <> from ->
+  0 <= from <= Z.of_nat addr ->
+  0 <= to <= Z.of_nat addr ->
+  transferRelation from to amt map map' ->
+  balanceOf_sum' map' addr acc  = balanceOf_sum' map addr acc.
+Proof.
+  intros map' Hneq Hleq1 Hleq2 Htransfer.
+  eapply transfer_burn_mint in Htransfer.
+  4: constructor.
+  remember (fun p : Z => if p =? from then map p - amt else map p) as imap.
+  destruct Htransfer.
+  - rewrite balanceOf_sum_mintTo with (map' := map') (map := imap) (to := to) (amt := amt); [ | lia | assumption ].
+    + rewrite leb_correct; [ | lia];
+      rewrite balanceOf_sum_burnFrom with (map' := imap) (map := map) (from := from) (amt := amt).
+        -- rewrite leb_correct; lia.
+        -- lia.
+        -- assumption.
+  - lia.
+  - lia.
+Qed.
+
+Lemma balances_after_transfer STATE src dst amount STATE' :
   0 <= src <= MAX_ADDRESS ->
   0 <= dst <= MAX_ADDRESS ->
   src <> dst ->
-  balanceOf_sum STATE =
-  balanceOf_sum (snd (transferFrom0 ENV STATE src dst amount)).
+  transferStateRelation src dst amount STATE STATE' ->
+  balanceOf_sum STATE = balanceOf_sum STATE' .
 Proof.
   intros. unfold balanceOf_sum; simpl.
-  erewrite <- transfer_thm.
+  apply Z.eq_sym_iff.
+  apply transfer_thm with (from := src) (to := dst) (amt := amount).
 
-  + unfold transfer, transfer_to, transfer_from.
-    convert_neq. rewrite_eqs. reflexivity.
-
-  + eauto.
-
-  + rewrite Z2Nat.id. assumption.
-    unfold MAX_ADDRESS. unfold UINT_MAX. lia.
-
-  + rewrite Z2Nat.id. assumption.
-    unfold MAX_ADDRESS. unfold UINT_MAX. lia.
+  + lia.
+  + lia.
+  + lia.
+  + destruct H2.
+    assumption.
 Qed.
 
-Lemma balances_after_burn ENV STATE src  amount :
+Lemma balances_after_burn STATE src  amount STATE' :
   0 <= src <= MAX_ADDRESS ->
+  burnStateRelation src amount STATE STATE' ->
   balanceOf_sum STATE - amount =
-  balanceOf_sum (snd (burnFrom0 ENV STATE src amount)).
+  balanceOf_sum STATE'.
 Proof.
   intros. unfold balanceOf_sum; simpl.
 
-  assert (forall map amt addr acc, src <= addr ->
-    balanceOf_sum' (transfer_from map src amt) (Z.to_nat addr) acc =
-    balanceOf_sum' map (Z.to_nat addr) acc - amt) as Htransfer_from.
-  { intros. rewrite balanceOf_sum_transfer_from.
+  assert (forall map amt addr acc map', src <= addr ->
+    burnRelation src amt map map' ->
+    balanceOf_sum' map' (Z.to_nat addr) acc =
+    balanceOf_sum' map (Z.to_nat addr) acc - amt) as HburnFrom.
+  { intros. rewrite balanceOf_sum_burnFrom with (map := map) (from := src) (amt := amt); [ | lia | assumption ].
 
     destruct (Z.to_nat src <=? Z.to_nat addr0)%nat eqn:Hleq.
     + reflexivity.
     + apply Nat.leb_nle in Hleq. lia.
-    + lia.
   }
 
-  erewrite <- Htransfer_from with (map := (balanceOf STATE)) (addr := MAX_ADDRESS) (amt := amount).
-  + reflexivity.
-  + lia.
+  rewrite Z.eq_sym_iff.
+  apply HburnFrom; [lia | ].
+  destruct H0.
+  assumption.
 Qed.
 
-Lemma balances_after_mint ENV STATE dst  amount :
+Lemma balances_after_mint STATE dst amount STATE':
   0 <= dst <= MAX_ADDRESS ->
+  mintStateRelation dst amount STATE STATE' ->
   balanceOf_sum STATE + amount =
-  balanceOf_sum (snd (mint0 ENV STATE dst amount)).
+  balanceOf_sum STATE'.
 Proof.
   intros. unfold balanceOf_sum; simpl.
 
-  assert (forall map amt addr acc, dst <= addr ->
-  balanceOf_sum' (transfer_to map dst amt) (Z.to_nat addr) acc =
-  balanceOf_sum' map (Z.to_nat addr) acc + amt).
-  { intros. rewrite balanceOf_sum_transfer_to.
+  assert (forall map amt addr acc map', dst <= addr ->
+  mintRelation dst amt map map' ->
+  balanceOf_sum' map' (Z.to_nat addr) acc =
+  balanceOf_sum' map (Z.to_nat addr) acc + amt) as HmintTo.
+  { intros. rewrite balanceOf_sum_mintTo with (map := map) (to := dst) (amt := amt); [ | lia | assumption ].
 
     destruct (Z.to_nat dst <=? Z.to_nat addr0)%nat eqn:Hleq.
     + reflexivity.
     + apply Nat.leb_nle in Hleq. lia.
-    + lia.
   }
 
-  erewrite <- H0 with (map := (balanceOf STATE)) (addr := MAX_ADDRESS) (amt := amount).
-  + reflexivity.
-  + lia.
+  rewrite Z.eq_sym_iff.
+  apply HmintTo; [lia | ].
+  destruct H0.
+  assumption.
 Qed.
 
-Theorem initialSupply': forall ENV _totalSupply (n : nat),
+Theorem initialSupply': forall ENV _totalSupply (n : nat), forall NA NA' STATE,
     0 <= Caller ENV ->
-    balanceOf_sum' (balanceOf (snd (Token ENV _totalSupply))) n 0 =
-    if (Z.of_nat n <? (Caller ENV)) then 0 else totalSupply (snd (Token ENV _totalSupply)).
+    constructor NA ENV _totalSupply STATE NA' ->
+    balanceOf_sum' (balanceOf STATE) n 0 =
+    if (Z.of_nat n <? (Caller ENV)) then 0 else totalSupply STATE.
 Proof.
-  intros.
-  unfold Token; simpl.
+  intros ENV ? ? ? ? ? ? Hcnstr.
+  destruct Hcnstr as [? Hinitprecs _ HnextNA]; simpl.
 
   assert (forall n : nat, Z.of_nat n < Caller ENV ->
       balanceOf_sum' (fun _binding_0 : address => if _binding_0 =? Caller ENV then _totalSupply else 0) n 0 = 0) as H0.
@@ -253,15 +344,14 @@ Proof.
   induction n.
   - simpl.
     destruct (Caller ENV) eqn:Hcaller.
-      + assert ( Z.of_nat 0 <? 0 = false).
+      + assert ( Z.of_nat 0 <? Caller ENV = false).
         * apply Z.ltb_ge. lia.
-        * rewrite H1. lia.
+        * rewrite <- Hcaller at 2. rewrite H1. lia.
       + reflexivity.
       + contradiction.
   - simpl. rewrite balanceOf_sum_acc.
     destruct (Z.of_nat (S n) <? Caller ENV) eqn:Hlt.
-    + destruct (Z.of_nat (S n) =? Caller ENV) eqn:Heq.
-      * lia.
+    + destruct (Z.of_nat (S n) =? Caller ENV) eqn:Heq. * lia.
       * rewrite H0.
         reflexivity.
         apply Zlt_is_lt_bool in Hlt. lia.
@@ -276,21 +366,23 @@ Proof.
         rewrite H1. lia.
 Qed.
 
-Theorem initialSupply: forall ENV _totalSupply,
+Theorem initialSupply: forall NA ENV _totalSupply STATE NA',
     0 <= Caller ENV <= MAX_ADDRESS ->
-    balanceOf_sum (snd (Token ENV _totalSupply)) =
-    totalSupply (snd (Token ENV _totalSupply)).
+    constructor NA ENV _totalSupply STATE NA' ->
+    balanceOf_sum STATE =
+    totalSupply STATE.
 Proof.
   intros.
   unfold balanceOf_sum.
-  rewrite -> initialSupply'.
-  unfold Token; simpl.
-  rewrite Z2Nat.id.
-  destruct (MAX_ADDRESS <? Caller ENV) eqn:Hineq.
-  + apply Z.ltb_lt in Hineq. lia.
-  + reflexivity.
-  + unfold MAX_ADDRESS. unfold UINT_MAX. lia.
-  + unfold MAX_ADDRESS. unfold UINT_MAX. lia.
+  erewrite -> initialSupply'.
+  - rewrite Z2Nat.id.
+    + destruct (MAX_ADDRESS <? Caller ENV) eqn:Hineq.
+      * destruct H0 as [? Hinit _ _].
+        apply Z.ltb_lt in Hineq. lia.
+      * rewrite Hineq. reflexivity.
+    + unfold MAX_ADDRESS. unfold UINT_MAX. lia.
+  - destruct H0 as [? Hinit _ _], Hinit. lia.
+  - eassumption.
 Qed.
 
 Theorem deltas: forall x1 x2 y1 y2,
@@ -307,9 +399,10 @@ Proof.
   destruct Hreach as [ BASE Hreach ], Hreach as [ Hinit Hmulti ].
 
   induction Hmulti as [ | STATE NEXT Hstep ].
-  - destruct Hinit as [ENV ? Hprecs].
-    apply initialSupply.
-    destruct Hprecs.
+  - destruct Hinit as [ENV ? ? ? Hcnstr].
+    eapply initialSupply.
+    2: eassumption.
+    destruct Hcnstr as [? Hinit _ _], Hinit.
     unfold MAX_ADDRESS.
     split; lia.
 
@@ -320,39 +413,147 @@ Proof.
     assert ( forall a b c,
       a - b = -c <-> a + c = b) as Ha4. lia.
 
-    destruct Hstep as [ENV Hextstep].
-    destruct Hextstep as [ENV STATE STATE' Hstep];
-    destruct Hstep; [ | assumption | | | | assumption | assumption | assumption | assumption | | | | | | assumption | assumption | assumption ];
-    (apply deltas with (x1 := balanceOf_sum STATE) (y1 := totalSupply STATE); [ assumption | simpl; destruct H ]).
-    + rewrite Z.sub_diag with (n := totalSupply STATE);
-      apply Zeq_minus;
-      apply (balances_after_transfer ENV); unfold MAX_ADDRESS; try split; lia.
-    + rewrite Z.sub_diag with (n := totalSupply STATE).
-      apply Zeq_minus.
-      apply (balances_after_transfer ENV); unfold MAX_ADDRESS; try split; lia.
-    + rewrite Z.sub_diag with (n := totalSupply STATE).
-      apply Zeq_minus.
-      apply (balances_after_transfer ENV); unfold MAX_ADDRESS; try split; lia.
-    + rewrite Z.sub_diag with (n := totalSupply STATE).
-      apply Zeq_minus.
-      assert (Hthm := balances_after_transfer ENV STATE).
-      unfold balanceOf_sum, transferFrom0, transferFrom2 in *.
-      apply Hthm; unfold MAX_ADDRESS; try split; lia.
-    + rewrite Ha1.
-      apply Ha2.
-      apply (balances_after_burn ENV). unfold MAX_ADDRESS; split; lia.
-    + rewrite Ha1.
-      apply Ha2.
-      apply (balances_after_burn ENV). unfold MAX_ADDRESS; split; lia.
-    + rewrite Ha1.
-      apply Ha2.
-      assert (Hthm := balances_after_burn ENV STATE).
-      unfold balanceOf_sum, burnFrom0, burnFrom1 in *.
-      apply Hthm. unfold MAX_ADDRESS; split; lia.
-    + rewrite Ha1.
-      apply Ha2.
-      apply (balances_after_burn ENV). unfold MAX_ADDRESS. split; lia.
-    + rewrite Ha3.
-      apply Ha4.
-      apply (balances_after_mint ENV). unfold MAX_ADDRESS. split; lia.
+    destruct Hstep as [NA [NA' [ENV Hextstep]]].
+    destruct Hextstep as [NA NA'  ENV STATE STATE' Hstep].
+    destruct Hstep.
+    + remember STATE' eqn:Hstate'.
+      destruct H.
+      * apply deltas with (x1 := balanceOf_sum STATE) (y1 := totalSupply STATE); [ assumption | simpl; destruct H ].
+        simpl.
+        rewrite Hstate'. unfold MAX_ADDRESS in *.
+        rewrite Z.sub_diag with (n := totalSupply STATE);
+        apply Zeq_minus;
+        eapply (balances_after_transfer) with (src := Caller ENV) (dst := to) (amount := _value); [ | |simpl |]. try split; unfold MAX_ADDRESS; try split; try lia. unfold MAX_ADDRESS. lia. lia.
+        constructor.
+        {
+          constructor.
+          - lia.
+          - intros p Hneq1 Hneq2.
+            rewrite <- Hstate'.
+            simpl. convert_neq. rewrite_eqs. reflexivity.
+          - rewrite <- Hstate'.
+            simpl. convert_neq. rewrite_eqs. rewrite Z.eqb_refl. lia.
+          - rewrite <- Hstate'.
+            simpl. convert_neq. rewrite_eqs. rewrite Z.eqb_refl. lia.
+            }
+      * simpl. rewrite <- IHHmulti. reflexivity.
+    + remember STATE' eqn:Hstate'.
+      destruct H.
+      * apply deltas with (x1 := balanceOf_sum STATE) (y1 := totalSupply STATE); [ assumption | simpl; destruct H ].
+        simpl.
+        rewrite Hstate'. unfold MAX_ADDRESS in *.
+        rewrite Z.sub_diag with (n := totalSupply STATE);
+        apply Zeq_minus;
+        eapply (balances_after_transfer) with (src := src) (dst := dst) (amount := amount); [ | |simpl |]. try split; unfold MAX_ADDRESS; try split; try lia. unfold MAX_ADDRESS. lia. lia.
+        constructor.
+        {
+          constructor.
+          - lia.
+          - intros p Hneq1 Hneq2.
+            rewrite <- Hstate'.
+            simpl. convert_neq. rewrite_eqs. reflexivity.
+          - rewrite <- Hstate'.
+            simpl. convert_neq. rewrite_eqs. rewrite Z.eqb_refl. lia.
+          - rewrite <- Hstate'. destruct H0.
+            simpl. convert_neq. rewrite_eqs. rewrite Z.eqb_refl. lia.
+            }
+      * apply deltas with (x1 := balanceOf_sum STATE) (y1 := totalSupply STATE); [ assumption | simpl; destruct H ].
+        simpl.
+        rewrite Hstate'. unfold MAX_ADDRESS in *.
+        rewrite Z.sub_diag with (n := totalSupply STATE);
+        apply Zeq_minus;
+        eapply (balances_after_transfer) with (src := src) (dst := dst) (amount := amount); [ | |simpl |]. try split; unfold MAX_ADDRESS; try split; try lia. unfold MAX_ADDRESS. lia. lia.
+        constructor.
+        {
+          constructor.
+          - lia.
+          - intros p Hneq1 Hneq2.
+            rewrite <- Hstate'.
+            simpl. convert_neq. rewrite_eqs. reflexivity.
+          - rewrite <- Hstate'.
+            simpl. convert_neq. rewrite_eqs. rewrite Z.eqb_refl. lia.
+          - rewrite <- Hstate'. destruct H0. destruct H0.
+            simpl. convert_neq. rewrite_eqs. rewrite Z.eqb_refl. lia.
+            }
+      * apply deltas with (x1 := balanceOf_sum STATE) (y1 := totalSupply STATE); [ assumption | simpl; destruct H ].
+        simpl.
+        rewrite Hstate'. unfold MAX_ADDRESS in *.
+        rewrite Z.sub_diag with (n := totalSupply STATE);
+        apply Zeq_minus;
+        eapply (balances_after_transfer) with (src := src) (dst := dst) (amount := amount); [ | |simpl |]. try split; unfold MAX_ADDRESS; try split; try lia. unfold MAX_ADDRESS. lia. lia.
+        constructor.
+        {
+          constructor.
+          - lia.
+          - intros p Hneq1 Hneq2.
+            rewrite <- Hstate'.
+            simpl. convert_neq. rewrite_eqs. reflexivity.
+          - rewrite <- Hstate'.
+            simpl. convert_neq. rewrite_eqs. rewrite Z.eqb_refl. lia.
+          - rewrite <- Hstate'. destruct H0. destruct H0.
+            simpl. convert_neq. rewrite_eqs. rewrite Z.eqb_refl. lia.
+            }
+      * simpl. rewrite <- IHHmulti at 2. reflexivity.
+      * simpl. rewrite <- IHHmulti at 2. reflexivity.
+    + destruct H; simpl; rewrite <- IHHmulti; unfold balanceOf_sum;  simpl; reflexivity.
+    + remember STATE' eqn:Hstate'.
+      destruct H.
+      * apply deltas with (x1 := balanceOf_sum STATE) (y1 := totalSupply STATE); [ assumption | simpl; destruct H ].
+        simpl.
+        rewrite Hstate'. unfold MAX_ADDRESS in *.
+        rewrite Ha1. rewrite Ha2.
+        eapply (balances_after_burn) with (src := Caller ENV) (amount := amount); [ unfold MAX_ADDRESS; split; lia | simpl ].
+        constructor.
+        constructor.
+        -- rewrite <- Hstate'; simpl. rewrite Z.eqb_refl. lia.
+        -- intros p Hneq.
+           rewrite <- Hstate'; simpl. convert_neq. rewrite_eqs. lia.
+    + remember STATE' eqn:Hstate'.
+      destruct H.
+      * apply deltas with (x1 := balanceOf_sum STATE) (y1 := totalSupply STATE); [ assumption | simpl; destruct H ].
+        rewrite Hstate'.
+        rewrite Ha1. rewrite Ha2.
+        eapply (balances_after_burn) with (src := src) (amount := amount); [ unfold MAX_ADDRESS; split; lia | simpl ].
+        constructor.
+        constructor.
+        -- rewrite <- Hstate'; simpl. rewrite Z.eqb_refl. lia.
+        -- intros p Hneq.
+           rewrite <- Hstate'; simpl. convert_neq. rewrite_eqs. lia.
+      * apply deltas with (x1 := balanceOf_sum STATE) (y1 := totalSupply STATE); [ assumption | simpl; destruct H ].
+        rewrite Hstate'.
+        rewrite Ha1. rewrite Ha2.
+        eapply (balances_after_burn) with (src := src) (amount := amount); [ unfold MAX_ADDRESS; split; lia | simpl ].
+        constructor.
+        constructor.
+        -- rewrite <- Hstate'; simpl. rewrite Z.eqb_refl. lia.
+        -- intros p Hneq.
+           rewrite <- Hstate'; simpl. convert_neq. rewrite_eqs. lia.
+      * apply deltas with (x1 := balanceOf_sum STATE) (y1 := totalSupply STATE); [ assumption | simpl; destruct H ].
+        rewrite Hstate'.
+        rewrite Ha1. rewrite Ha2.
+        eapply (balances_after_burn) with (src := src) (amount := amount); [ unfold MAX_ADDRESS; split; lia | simpl ].
+        constructor.
+        constructor.
+        -- rewrite <- Hstate'; simpl. rewrite Z.eqb_refl. lia.
+        -- intros p Hneq.
+           rewrite <- Hstate'; simpl. convert_neq. rewrite_eqs. lia.
+    + remember STATE' eqn:Hstate'.
+      destruct H.
+      * apply deltas with (x1 := balanceOf_sum STATE) (y1 := totalSupply STATE); [ assumption | simpl; destruct H ].
+        rewrite Hstate'.
+        rewrite Ha3. rewrite Ha4.
+        eapply (balances_after_mint) with (dst := dst) (amount := amount); [ unfold MAX_ADDRESS; split; lia | simpl ].
+        constructor.
+        constructor.
+        -- rewrite <- Hstate'; simpl. rewrite Z.eqb_refl. lia.
+        -- intros p Hneq.
+           rewrite <- Hstate'; simpl. convert_neq. rewrite_eqs. lia.
+    + remember STATE' eqn:Hstate'.
+      destruct H.
+      * apply deltas with (x1 := balanceOf_sum STATE) (y1 := totalSupply STATE); [ assumption | simpl; destruct H ].
+        rewrite Hstate'. rewrite Z.sub_diag with (n := totalSupply STATE).
+        apply Zeq_minus.
+        rewrite <- Hstate'; simpl. unfold balanceOf_sum;  simpl; reflexivity.
+    + destruct H. simpl. unfold balanceOf_sum. rewrite <- IHHmulti.  simpl; reflexivity.
+    + destruct H. simpl. unfold balanceOf_sum. rewrite <- IHHmulti.  simpl; reflexivity.
 Qed.
