tests/coq/safemath/Theory.v
@@ -7,27 +7,27 @@ Open Scope Z_scope.
 Import SafeMath.
 
 (* trivial observation that there is only one possible state *)
-Lemma state_constant : forall s, exists a, s = state a.
+Lemma state_constant : forall s, exists addr a, s = state addr a.
 Proof.
   intros.
   destruct s.
-  exists addr0.
+  exists addr0, BALANCE0.
   reflexivity.
 Qed.
 
-Theorem mul_correct : forall e s x y,
-  nextAddrConstraint e s ->
-  range256 x /\ range256 y /\ range256 (x * y) <-> mul0_ret e s x y (x * y).
+Theorem mul_correct : forall na e s x y,
+  mul_conds na e s x y ->
+  range256 x /\ range256 y /\ range256 (x * y) <-> mul0_ret na e s x y (x * y).
 Proof.
   intros.
   split. {
     intros.
+    destruct H.
     destruct H0 as [Hx [Hy Hxy]].
     unfold range256 in *.
     apply mul0_ret_intro.
     - constructor;
-      repeat split; try lia.
-      assumption.
+      repeat split; try lia. assumption.
     - trivial.
   } {
     intros Hmul_ret. destruct Hmul_ret. destruct H0.
@@ -37,8 +37,8 @@ Qed.
 
 
 Theorem mul_is_mul :
-  forall e s x y z,
-    mul0_ret e s x y z ->
+  forall na e s x y z,
+    mul0_ret na e s x y z ->
     z = x * y.
 Proof.
   intros. inversion H.
